some work on Cevaluate_any_env
changed statement to include syneq stuff in the induction (along with
restricting and extending the environment). (includes failed attempt to
prove the syneq stuff on its own.) up to let case.

also fixed up syneq_refl since :Cv induction changed when it was
decoupled from :Cexp.

examples/miniML/compiler/correctness/intLangScript.sml
@@ -633,16 +633,17 @@ val _ = export_rewrites["CevalPrim2_free_vars"]
 val syneq_cases = CompileTheory.syneq_cases
 val syneq_ind = CompileTheory.syneq_ind
 
-val rel_result_def = Define`
-rel_result R r1 r2 = (∃e. (r1 = Rerr e) ∧ (r2 = Rerr e)) ∨
-                     (∃v1 v2. (r1 = Rval v1) ∧ (r2 = Rval v2) ∧ R v1 v2)`
+val result_rel_def = Define`
+(result_rel R (Rval v1) (Rval v2) = R v1 v2) ∧
+(result_rel R (Rerr e1) (Rerr e2) = (e1 = e2)) ∧
+(result_rel R _ _ = F)`
+val _ = export_rewrites["result_rel_def"]
 
 val syneq_refl = store_thm(
 "syneq_refl",
 ``∀x. syneq x x``,
 (TypeBase.induction_of``:Cv``)
-|> Q.SPECL [`K T`,`W syneq`,`K T`,`K T`,`EVERY (W syneq o SND)`]
-|> Q.SPECL [`W syneq o SND`,`K T`,`K T`,`K T`,`EVERY (W syneq)`]
+|> Q.SPECL [`W syneq`,`EVERY ((W syneq) o SND)`,`W syneq o SND`,`EVERY (W syneq)`]
 |> SIMP_RULE(srw_ss())[]
 |> UNDISCH_ALL
 |> CONJUNCT1
@@ -699,11 +700,263 @@ rw[syneq_cases] >- (
             optionTheory.NOT_SOME_NONE,
             optionTheory.SOME_11] ))
 
+val result_rel_syneq_refl = store_thm(
+"result_rel_syneq_refl",
+``∀x. result_rel syneq x x``,
+Cases >> rw[])
+val _ = export_rewrites["result_rel_syneq_refl"]
+
+val result_rel_Rval = store_thm(
+"result_rel_Rval",
+``result_rel R (Rval v) r = ∃v'. (r = Rval v') ∧ R v v'``,
+Cases_on `r` >> rw[])
+val result_rel_Rerr = store_thm(
+"result_rel_Rerr",
+``result_rel R (Rerr e) r = (r = Rerr e)``,
+Cases_on `r` >> rw[EQ_IMP_THM])
+val _ = export_rewrites["result_rel_Rval","result_rel_Rerr"]
+
+val Cmatch_result_rel_def = Define`
+  (Cmatch_result_rel R (Cmatch e1) (Cmatch e2) = R e1 e2) ∧
+  (Cmatch_result_rel R Cno_match r = (r = Cno_match)) ∧
+  (Cmatch_result_rel R Cmatch_error r = (r = Cmatch_error)) ∧
+  (Cmatch_result_rel R _ _ = F)`
+val _ = export_rewrites["Cmatch_result_rel_def"]
+
+val fmap_rel_def = Define`
+  fmap_rel R f1 f2 = (FDOM f2 = FDOM f1) ∧ (∀x. x ∈ FDOM f1 ⇒ R (f1 ' x) (f2 ' x))`
+
+val fmap_rel_FUPDATE_same = store_thm(
+"fmap_rel_FUPDATE_same",
+``fmap_rel R f1 f2 ∧ R v1 v2 ⇒ fmap_rel R (f1 |+ (k,v1)) (f2 |+ (k,v2))``,
+rw[fmap_rel_def,FAPPLY_FUPDATE_THM] >> rw[])
+
+val fmap_rel_FUPDATE_LIST_same = store_thm(
+"fmap_rel_FUPDATE_LIST_same",
+``∀R ls1 ls2 f1 f2.
+  fmap_rel R f1 f2 ∧ (MAP FST ls1 = MAP FST ls2) ∧ (LIST_REL R (MAP SND ls1) (MAP SND ls2))
+  ⇒ fmap_rel R (f1 |++ ls1) (f2 |++ ls2)``,
+gen_tac >>
+Induct >> Cases >> rw[FUPDATE_LIST_THM,LIST_REL_CONS1] >>
+Cases_on `ls2` >> fs[FUPDATE_LIST_THM] >>
+first_x_assum match_mp_tac >> fs[] >> rw[] >>
+qmatch_assum_rename_tac `R a (SND b)`[] >>
+Cases_on `b` >> fs[] >>
+rw[fmap_rel_FUPDATE_same])
+
+val fmap_rel_FEMPTY = store_thm(
+"fmap_rel_FEMPTY",
+``fmap_rel R FEMPTY FEMPTY``,
+rw[fmap_rel_def])
+val _ = export_rewrites["fmap_rel_FEMPTY"]
+
+(* TODO: move *)
+val LIST_REL_EVERY_ZIP = store_thm(
+"LIST_REL_EVERY_ZIP",
+``!R l1 l2. LIST_REL R l1 l2 = ((LENGTH l1 = LENGTH l2) /\ EVERY (UNCURRY R) (ZIP (l1,l2)))``,
+GEN_TAC THEN Induct THEN SRW_TAC[][LENGTH_NIL_SYM] THEN
+SRW_TAC[][EQ_IMP_THM,LIST_REL_CONS1] THEN SRW_TAC[][] THEN
+Cases_on `l2` THEN FULL_SIMP_TAC(srw_ss())[])
+
+val Cpmatch_syneq = store_thm(
+"Cpmatch_syneq",
+``(∀env1 p v1 env2 v2.
+   fmap_rel syneq env1 env2 ∧ syneq v1 v2 ⇒
+     Cmatch_result_rel (fmap_rel syneq)
+       (Cpmatch env1 p v1) (Cpmatch env2 p v2)) ∧
+  (∀env1 ps vs1 env2 vs2.
+   fmap_rel syneq env1 env2 ∧ LIST_REL syneq vs1 vs2 ⇒
+     Cmatch_result_rel (fmap_rel syneq)
+       (Cpmatch_list env1 ps vs1) (Cpmatch_list env2 ps vs2))``,
+ho_match_mp_tac Cpmatch_ind >>
+strip_tac >- (
+  rw[Cpmatch_def,fmap_rel_FUPDATE_same] ) >>
+strip_tac >- (
+  ntac 4 gen_tac >>
+  Cases >> rw[Cpmatch_def,syneq_cases] ) >>
+strip_tac >- (
+  rpt gen_tac >> strip_tac >> gen_tac >>
+  Cases >> rw[Cpmatch_def,syneq_cases,EVERY2_EVERY] >>
+  pop_assum (match_mp_tac o MP_CANON) >>
+  rw[LIST_REL_EVERY_ZIP] ) >>
+strip_tac >- (
+  ntac 5 gen_tac >>
+  Cases >> rw[Cpmatch_def,syneq_cases] ) >>
+strip_tac >- (
+  rw[Cpmatch_def,syneq_cases] >>
+  rw[Cpmatch_def]) >>
+strip_tac >- (
+  rw[Cpmatch_def,syneq_cases] >>
+  rw[Cpmatch_def]) >>
+strip_tac >- (
+  rw[Cpmatch_def,syneq_cases] ) >>
+strip_tac >- (
+  rw[Cpmatch_def,syneq_cases] >>
+  rw[Cpmatch_def]) >>
+strip_tac >- (
+  rw[Cpmatch_def,syneq_cases] >>
+  rw[Cpmatch_def]) >>
+strip_tac >- (
+  rw[Cpmatch_def]) >>
+strip_tac >- (
+  rw[Cpmatch_def,LIST_REL_CONS1] >>
+  rw[Cpmatch_def] >>
+  Cases_on `Cpmatch env1 p v1` >> fs[] >>
+  qmatch_assum_rename_tac `syneq v1 v2`[] >>
+  first_x_assum (qspecl_then [`env2`,`v2`] mp_tac) >>
+  Cases_on `Cpmatch env2 p v2` >> rw[Cmatch_result_rel_def]) >>
+strip_tac >- (
+  rw[Cpmatch_def,LIST_REL_CONS1] >>
+  rw[Cpmatch_def] ) >>
+rw[Cpmatch_def])
+
+(*
+val Cevaluate_syneq_env = store_thm(
+"Cevaluate_syneq_env",
+``∀env exp res. Cevaluate env exp res ⇒
+  ∀env'. fmap_rel syneq env env'
+    ⇒ ∃res'. Cevaluate env' exp res' ∧ result_rel syneq res res'``,
+ho_match_mp_tac Cevaluate_nice_ind >>
+strip_tac >- rw[] >>
+strip_tac >- rw[fmap_rel_def] >>
+strip_tac >- rw[] >>
+strip_tac >- (
+  rw[Cevaluate_con,Cevaluate_list_with_Cevaluate,
+     Cevaluate_list_with_value] >>
+  fsrw_tac[DNF_ss][] >>
+  qpat_assum `∀n env'. n < LENGTH es ⇒ X` (fn th => th
+    |> SIMP_RULE(srw_ss())[Once SWAP_FORALL_THM]
+    |> qspec_then`env'` mp_tac) >> rw[] >>
+  fs[GSYM RIGHT_EXISTS_IMP_THM] >>
+  fs[Once SKOLEM_THM] >>
+  qexists_tac `GENLIST f (LENGTH vs)` >> fs[] >>
+  rw[Once syneq_cases,EVERY2_EVERY,EVERY_MEM,pairTheory.FORALL_PROD,MEM_ZIP] >>
+  rw[EL_GENLIST] ) >>
+strip_tac >- (
+  map_every qx_gen_tac [`env`,`m`] >>
+  rw[Cevaluate_con,Cevaluate_list_with_Cevaluate,
+     Cevaluate_list_with_error] >>
+  qexists_tac `n` >> fs[] >>
+  qx_gen_tac `m` >> strip_tac >>
+  first_x_assum (qspec_then `m` mp_tac) >> rw[] >>
+  pop_assum (qspec_then `env'` mp_tac) >>
+  rw[] >> PROVE_TAC[] ) >>
+strip_tac >- (
+  rw[Cevaluate_tageq] >>
+  fsrw_tac[DNF_ss][] >>
+  qexists_tac `m` >> fs[] >>
+  first_x_assum (qspec_then `env'` mp_tac) >>
+  fs[] >> rw[syneq_cases] >> PROVE_TAC[] ) >>
+strip_tac >- rw[Cevaluate_tageq] >>
+strip_tac >- (
+  ntac 3 gen_tac >>
+  qx_gen_tac `m` >>
+  rw[Cevaluate_proj] >>
+  fsrw_tac[DNF_ss][] >>
+  qexists_tac `m` >> fs[] >>
+  first_x_assum (qspec_then `env'` mp_tac) >>
+  fs[] >> rw[Once syneq_cases] >>
+  pop_assum mp_tac >>
+  fsrw_tac[DNF_ss][GSYM AND_IMP_INTRO,EVERY2_EVERY,EVERY_MEM,MEM_EL,LENGTH_ZIP,EL_ZIP] >> PROVE_TAC[] ) >>
+strip_tac >- rw[Cevaluate_proj] >>
+strip_tac >- rw[] >>
+strip_tac >- (
+  rw[Cevaluate_mat_cons] >>
+  fsrw_tac[DNF_ss][] >>
+  qmatch_assum_rename_tac `fmap_rel syneq env1 env2` [] >>
+  qmatch_assum_rename_tac `Cpmatch env1 p (env1 ' k) = Cmatch env3` [] >>
+  qspecl_then [`env1`,`p`,`env1 ' k`,`env2`,`env2 ' k`] mp_tac  (CONJUNCT1 Cpmatch_syneq) >>
+  `syneq (env1 ' k) (env2 ' k)` by fs[fmap_rel_def] >>
+  Cases_on `Cpmatch env2 p (env2 ' k)` >> rw[Cmatch_result_rel_def] >>
+  fs[fmap_rel_def] ) >>
+strip_tac >- (
+  rw[Cevaluate_mat_cons] >>
+  fsrw_tac[DNF_ss][] >>
+  qmatch_assum_rename_tac `fmap_rel syneq env1 env2` [] >>
+  qmatch_assum_rename_tac `Cpmatch env1 p (env1 ' k) = Cno_match` [] >>
+  qspecl_then [`env1`,`p`,`env1 ' k`,`env2`,`env2 ' k`] mp_tac  (CONJUNCT1 Cpmatch_syneq) >>
+  `syneq (env1 ' k) (env2 ' k)` by fs[fmap_rel_def] >>
+  Cases_on `Cpmatch env2 p (env2 ' k)` >> rw[Cmatch_result_rel_def] >>
+  fs[fmap_rel_def] ) >>
+strip_tac >- rw[] >>
+strip_tac >- (
+  rw[Cevaluate_let_cons] >>
+  fsrw_tac[DNF_ss][] >>
+  res_tac >> rw[] >>
+  disj1_tac >>
+  rw[Once SWAP_EXISTS_THM] >>
+  qmatch_assum_rename_tac `syneq v1 v2`[] >>
+  qexists_tac`v2` >>
+  rw[] >>
+  first_x_assum match_mp_tac >>
+  rw[fmap_rel_FUPDATE_same] ) >>
+strip_tac >- rw[Cevaluate_let_cons] >>
+strip_tac >- (
+  rw[] >>
+  rw[Once Cevaluate_cases] >>
+  first_x_assum match_mp_tac >>
+  rw[FOLDL2_FUPDATE_LIST_paired] >>
+  match_mp_tac fmap_rel_FUPDATE_LIST_same >>
+  fs[MAP2_MAP,MAP_ZIP] >>
+  fs[LIST_REL_EVERY_ZIP,MAP_ZIP,ZIP_MAP,LENGTH_ZIP,EVERY_MAP] >>
+  rw[EVERY_MEM,MEM_ZIP,pairTheory.UNCURRY] >>
+  rw[syneq_cases,FLOOKUP_DEF] >>
+  fs[fmap_rel_def] >>
+  rw[] >> rw[optionTheory.OPTREL_def] ) >>
+strip_tac >- (
+  rw[] >>
+  rw[Once Cevaluate_cases] >>
+  first_x_assum match_mp_tac >>
+  rw[FOLDL_FUPDATE_LIST] >>
+  match_mp_tac fmap_rel_FUPDATE_LIST_same >>
+  fs[MAP_MAP_o,combinTheory.o_DEF] >>
+  rw[LIST_REL_EL_EQN,EL_MAP] >>
+  rw[syneq_cases,EVERY_MEM,pairTheory.UNCURRY] >>
+  fs[FLOOKUP_DEF] >>
+  fs[fmap_rel_def] >>
+  rw[] >> rw[optionTheory.OPTREL_def] ) >>
+strip_tac >- (
+  rw[syneq_cases] >>
+  fs[fmap_rel_def] >>
+  fs[FLOOKUP_DEF] >>
+  rw[] >> rw[optionTheory.OPTREL_def] ) >>
+strip_tac >- (
+  rw[] >>
+  rw[Once Cevaluate_cases] >>
+  fsrw_tac[DNF_ss][] >>
+  disj1_tac >>
+  fs[Cevaluate_list_with_Cevaluate,Cevaluate_list_with_value] >>
+  fsrw_tac[DNF_ss][] >>
+  qmatch_assum_rename_tac `fmap_rel syneq env1 env2`[] >>
+  qpat_assum `∀e''. P ⇒ ∃v'. Q ∧ syneq x y` (qspec_then `env2` mp_tac) >>
+  rw[syneq_cases] >>
+  qmatch_assum_rename_tac `Cevaluate env2 exp (Rval (CClosure env3 ns b))`[] >>
+  CONV_TAC (RESORT_EXISTS_CONV (fn ls => tl ls @ [hd ls])) >>
+  map_every qexists_tac [`env3`,`ns`,`b`] >>
+  fsrw_tac[DNF_ss][RIGHT_FORALL_IMP_THM,Once SWAP_FORALL_THM] >>
+  qpat_assum `∀env' n. P` (qspec_then `env2` mp_tac) >> fs[] >>
+  disch_then(mp_tac o SIMP_RULE(srw_ss())[GSYM RIGHT_EXISTS_IMP_THM,SKOLEM_THM]) >>
+  rw[] >>
+  qexists_tac `GENLIST f (LENGTH vs)` >>
+  fs[] >>
+  qpat_assum `LENGTH ns = LENGTH vs` assume_tac >>
+  fs[FOLDL2_FUPDATE_LIST,MAP2_MAP,FST_pair,MAP_ZIP,SND_pair] >>
+
+  first_x_assum match_mp_tac >>
+  match_mp_tac fmap_rel_FUPDATE_LIST_same >>
+  rw[MAP_ZIP,LIST_REL_EL_EQN,LENGTH_ZIP] >>
+*)
+
+val fmap_rel_FUNION_rels = store_thm(
+"fmap_rel_FUNION_rels",
+``fmap_rel R f1 f2 ∧ fmap_rel R f3 f4 ⇒ fmap_rel R (f1 ⊌ f3) (f2 ⊌ f4)``,
+rw[fmap_rel_def,FUNION_DEF] >> rw[])
+
 val final0 =
   qsuff_tac `env0 ⊌ env1 = env1` >- PROVE_TAC[] >>
   rw[GSYM SUBMAP_FUNION_ABSORPTION] >>
   rw[Abbr`env0`,Abbr`env1`,SUBMAP_DEF,DRESTRICT_DEF,FUNION_DEF,FUN_FMAP_DEF,pairTheory.UNCURRY,FAPPLY_FUPDATE_THM] >>
-  fsrw_tac[boolSimps.DNF_ss,SATISFY_ss][FUN_FMAP_DEF,pairTheory.UNCURRY,MEM_EL] >>
+  fsrw_tac[boolSimps.DNF_ss,SATISFY_ss][FUN_FMAP_DEF,pairTheory.UNCURRY,MEM_EL,fmap_rel_def] >>
   metis_tac[]
 
 val final =
@@ -711,32 +964,31 @@ val final =
   qmatch_abbrev_tac `Cevaluate env1 ee rr` >>
   final0
 
-val rel_result_syneq_refl = store_thm(
-"rel_result_syneq_refl",
-``∀x. rel_result syneq x x``,
-Cases >> rw[rel_result_def])
-val _ = export_rewrites["rel_result_syneq_refl"]
-
 (*
 val Cevaluate_any_env = store_thm(
 "Cevaluate_any_env",
 ``∀env exp res. Cevaluate env exp res ⇒
   free_vars exp ⊆ FDOM env ⇒
-    ∀env'. ∃res'. Cevaluate ((DRESTRICT env (free_vars exp)) ⊌ env') exp res' ∧ (rel_result syneq) res res'``,
+    ∀env'. fmap_rel syneq env env' ⇒
+      ∀env''. ∃res'.
+        Cevaluate ((DRESTRICT env' (free_vars exp)) ⊌ env'') exp res' ∧ (result_rel syneq) res res'``,
 ho_match_mp_tac Cevaluate_nice_ind >>
 strip_tac >- rw[] >>
-strip_tac >- rw[DRESTRICT_DEF,FUNION_DEF] >>
+strip_tac >- rw[DRESTRICT_DEF,FUNION_DEF,fmap_rel_def] >>
 strip_tac >- rw[] >>
 strip_tac >- (
   rw[Cevaluate_con,Cevaluate_list_with_Cevaluate,
      Cevaluate_list_with_value,FOLDL_UNION_BIGUNION] >>
-  fsrw_tac[DNF_ss,SATISFY_ss][SUBSET_DEF,MEM_EL,rel_result_def] >>
+  fsrw_tac[DNF_ss,SATISFY_ss][SUBSET_DEF,MEM_EL,result_rel_def] >>
   rw[syneq_cases,EVERY2_EVERY,EVERY_MEM] >>
   rw[pairTheory.FORALL_PROD] >>
-  Q.PAT_ABBREV_TAC `env1 = X ⊌ env'` >>
-  qpat_assum `∀n env'. n < LENGTH es ⇒ X` (fn th => th
+  Q.PAT_ABBREV_TAC `env1 = X ⊌ env''` >>
+  qpat_assum `∀n env' env''. n < LENGTH es ⇒ X` (fn th => th
     |> SIMP_RULE(srw_ss())[Once SWAP_FORALL_THM]
-    |> qspec_then`env1` assume_tac) >>
+    |> Q.SPEC `env'`
+    |> SIMP_RULE(srw_ss())[Once SWAP_FORALL_THM]
+    |> qspec_then`env1` mp_tac) >>
+  rw[] >>
   fs[GSYM RIGHT_EXISTS_IMP_THM] >>
   fs[Once SKOLEM_THM] >>
   fsrw_tac[DNF_ss][] >>
@@ -752,43 +1004,47 @@ strip_tac >- (
   rw[Cevaluate_con,Cevaluate_list_with_Cevaluate,
      Cevaluate_list_with_error,FOLDL_UNION_BIGUNION] >>
   qpat_assum `n < LENGTH es` assume_tac >>
-  fsrw_tac[DNF_ss,SATISFY_ss][SUBSET_DEF,MEM_EL,rel_result_def] >>
+  fsrw_tac[DNF_ss,SATISFY_ss][SUBSET_DEF,MEM_EL,result_rel_def] >>
   qexists_tac `n` >> fs[] >>
-  conj_tac >- final >>
+  first_x_assum (qspec_then `env'` mp_tac) >> fs[] >>
+  strip_tac >> conj_tac  >- final >>
   qx_gen_tac `m` >> strip_tac >>
   first_x_assum (qspec_then `m` mp_tac) >>
   `m < LENGTH es` by srw_tac[ARITH_ss][] >>
   fsrw_tac[DNF_ss,SATISFY_ss][SUBSET_DEF,MEM_EL] >>
   rw[] >>
-  Q.PAT_ABBREV_TAC `env1 = X ⊌ env'` >>
-  first_x_assum (qspec_then `env1` mp_tac) >>
+  Q.PAT_ABBREV_TAC `env1 = X ⊌ env''` >>
+  first_x_assum (qspecl_then [`env'`,`env1`] mp_tac) >>
   rw[] >>
   qmatch_assum_abbrev_tac `Cevaluate (env0 ⊌ env1) ee rr` >>
+  qmatch_assum_rename_tac `syneq v v2`[] >>
   qexists_tac `v2` >> final0) >>
 strip_tac >- (
   rw[Cevaluate_tageq] >>
-  fsrw_tac[DNF_ss][rel_result_def] >>
+  fsrw_tac[DNF_ss][result_rel_def] >>
   qexists_tac `m` >> fs[] >>
   fs[syneq_cases] >>
   PROVE_TAC[]) >>
-strip_tac >- rw[Cevaluate_tageq,rel_result_def] >>
+strip_tac >- rw[Cevaluate_tageq,result_rel_def] >>
 strip_tac >- (
   rw[Cevaluate_proj] >>
-  fsrw_tac[DNF_ss][rel_result_def] >>
+  fsrw_tac[DNF_ss][result_rel_def] >>
   qmatch_abbrev_tac `X` >>
   qpat_assum `∀env'. X` mp_tac >>
   rw[syneq_cases] >> unabbrev_all_tac >>
   qexists_tac `m` >>
+  pop_assum (qspec_then `env'` mp_tac) >> rw[] >>
   fsrw_tac[DNF_ss][EVERY2_EVERY,EVERY_MEM,MEM_EL,SKOLEM_THM] >>
   pop_assum mp_tac >> fs[LENGTH_ZIP,EL_ZIP] >>
   PROVE_TAC[]) >>
-strip_tac >- rw[Cevaluate_proj,rel_result_def] >>
+strip_tac >- rw[Cevaluate_proj,result_rel_def] >>
 strip_tac >- rw[] >>
 strip_tac >- (
   rw[Cevaluate_mat_cons,FOLDL_UNION_BIGUNION_paired,
      DRESTRICT_DEF,FUNION_DEF] >>
   fsrw_tac[DNF_ss][] >>
-  disj1_tac >>
+  disj1_tac >> disj1_tac >>
+  `n ∈ FDOM env''` by fs[fmap_rel_def] >> fs[] >>
   fs[Once Cpmatch_FEMPTY] >>
   Cases_on `Cpmatch FEMPTY p (env ' n)` >> fs[] >>
   rw[] >>
@@ -796,21 +1052,34 @@ strip_tac >- (
   fsrw_tac[DNF_ss,SATISFY_ss][SUBSET_DEF,pairTheory.FORALL_PROD] >>
   `∀x. x ∈ free_vars exp ⇒ x ∈ Cpat_vars p ∨ x ∈ FDOM env` by
     PROVE_TAC[] >> fs[] >>
-  Q.PAT_ABBREV_TAC `env1 = f ⊌ (X ⊌ env'')` >>
-  first_x_assum (qspec_then `env1` mp_tac) >>
-  rw[] >>
+  `Cmatch_result_rel (fmap_rel syneq) (Cpmatch FEMPTY p (env ' n)) (Cpmatch FEMPTY p (env'' ' n))` by (
+    match_mp_tac (CONJUNCT1 Cpmatch_syneq) >>
+    fs[fmap_rel_def] ) >>
+  pop_assum mp_tac >>
+  Cases_on `Cpmatch FEMPTY p (env'' ' n)` >> rw[] >>
+  qmatch_assum_rename_tac `Cpmatch FEMPTY p (env'' ' n) = Cmatch env2` [] >>
+  Q.PAT_ABBREV_TAC `env1 = env2 ⊌ (X ⊌ env''')` >>
+  qmatch_assum_rename_tac `Cpmatch FEMPTY p (env ' n) = Cmatch env4` [] >>
+  first_x_assum (qspecl_then [`env2 ⊌ env''`,`env1`] mp_tac) >>
+  rw[fmap_rel_FUNION_rels] >>
   qmatch_assum_abbrev_tac `Cevaluate (env0 ⊌ env1) ee rr` >>
   qexists_tac `rr` >> final0) >>
 strip_tac >- (
   rw[Cevaluate_mat_cons,FOLDL_UNION_BIGUNION_paired,
      DRESTRICT_DEF,FUNION_DEF] >>
   fsrw_tac[DNF_ss][] >>
-  disj2_tac >>
+  disj1_tac >> disj2_tac >>
+  `n ∈ FDOM env'` by fs[fmap_rel_def] >> fs[]
   fs[Once Cpmatch_FEMPTY] >>
   Cases_on `Cpmatch FEMPTY p (env ' n)` >> fs[] >>
   qpat_assum `n ∈ FDOM env` assume_tac >> fs[] >>
-  Q.PAT_ABBREV_TAC `env1 = (X ⊌ env')` >>
-  first_x_assum (qspec_then `env1` mp_tac) >>
+  `Cmatch_result_rel (fmap_rel syneq) (Cpmatch FEMPTY p (env ' n)) (Cpmatch FEMPTY p (env' ' n))` by (
+    match_mp_tac (CONJUNCT1 Cpmatch_syneq) >>
+    fs[fmap_rel_def] ) >>
+  pop_assum mp_tac >>
+  Cases_on `Cpmatch FEMPTY p (env' ' n)` >> rw[] >>
+  Q.PAT_ABBREV_TAC `env1 = (X ⊌ env'')` >>
+  first_x_assum (qspecl_then [`env'`,`env1`] mp_tac) >>
   rw[] >>
   qmatch_assum_abbrev_tac `Cevaluate (env0 ⊌ env1) ee rr` >>
   qexists_tac `rr` >> final0) >>
@@ -824,24 +1093,29 @@ strip_tac >- (
   qx_gen_tac `env'` >>
   disj1_tac >>
   Q.PAT_ABBREV_TAC `env1 = X ⊌ env'` >>
-  qpat_assum `∀env'. ∃res'. X ∧ rel_result syneq (Rval v) res'`
+  qpat_assum `∀env'. ∃v'. X ∧ syneq v v'`
     (qspec_then `env1` mp_tac) >>
   rw[] >>
   rw[Once SWAP_EXISTS_THM] >>
   qmatch_assum_abbrev_tac `Cevaluate (env0 ⊌ env1) ee rr` >>
-  `∃v'. rr = Rval v'` by (
-    Cases_on `rr` >> fs[rel_result_def] ) >>
-  qexists_tac `v'` >>
+  qmatch_assum_rename_tac `syneq v v2`[] >>
+  qexists_tac `v2` >>
   simp_tac(srw_ss())[RIGHT_EXISTS_AND_THM,GSYM CONJ_ASSOC] >>
   conj_tac >- final0 >>
   `∀x. x ∈ free_vars b ∧ ¬MEM x ns ⇒ (x = n) ∨ x ∈ FDOM env` by (
     PROVE_TAC[] ) >> fs[] >>
+  qsuff_tac `∃r. Cevaluate (env1 |+ (n,v)) (CLet ns es b) r ∧ result_rel syneq res r` >- (
 
-  need lemma about allowing syneq values in an environment to get a syneq Cevaluate result
-
-  Cases_on `n ∈ free_vars b ∧ ¬MEM n ns ∨
-            ∃x. n ∈ free_vars x ∧ MEM x es` >> fs[] >>
-  final ) >>
+    ) >>
+  first_x_assum (qspec_then `env1 |+ (n,v)` mp_tac) >>
+  rw[] >>
+  qmatch_assum_rename_tac `result_rel syneq res r`[] >>
+  qexists_tac `r` >> fs[] >>
+  qunabbrev_tac `env1` >>
+  Q.PAT_ABBREV_TAC `env1 = X |+ (n,v)` >>
+  qunabbrev_tac `env0` >>
+  qmatch_assum_abbrev_tac `Cevaluate (env0 ⊌ env1) (CLet ns es b) r` >>
+  final0 ) >>
 strip_tac >- (
   rw[Cevaluate_let_cons,FOLDL_UNION_BIGUNION] >>
   disj2_tac >> fs[] >>
